theories/Eq/SSimTheory.v
@@ -1,0 +1,580 @@
+From Coq Require Import Lia Basics Fin.
+
+From Coinduction Require Import
+     coinduction rel tactics.
+
+From ITree Require Import Core.Subevent.
+
+From CTree Require Import
+     CTree
+     Utils
+     Eq.Equ
+     Eq.SBisim
+     Eq.Shallow
+     Eq.Trans.
+
+From RelationAlgebra Require Export
+     rel srel.
+
+Set Implicit Arguments.
+
+Import SBisimNotations.
+
+(* TODO: Decide where to set this *)
+Arguments trans : simpl never.
+
+Section ssim_theory.
+
+  Context {E F C D : Type -> Type} {X Y : Type}.
+  Context `{HasStuck : C0 -< C} `{HasStuck' : C0 -< D}.
+  Notation ss1 := (@ss E E C C X X _ _).
+  Notation sse := (ss1 eq).
+  Notation ss := (@ss E F C D X Y).
+  Notation ssim1  := (@ssim E E C C X X).
+  Notation ssim  := (@ssim E F C D X Y).
+  Notation sst L := (coinduction.t (ss L)).
+  Notation ssbt L := (coinduction.bt (ss L)).
+  Notation ssT L := (coinduction.T (ss L)).
+
+  Lemma Reflexive_ss: forall R, Reflexive R -> Reflexive (sse R).
+  Proof.
+    intros R H t l t' tt'.
+    exists t', l. auto.
+  Qed.
+
+  #[global] Instance Reflexive_ssim: Reflexive (ssim1 eq).
+  Proof.
+    cbn. coinduction R CH.
+    apply Reflexive_ss. cbn. apply CH.
+  Qed.
+
+  Lemma Transitive_ss: forall R, Transitive R -> Transitive (sse R).
+  Proof.
+    intros R H x y z xy yz l x' xx'.
+    destruct (xy _ _ xx') as (y' & ? & yy' & x'y' & <-).
+    destruct (yz _ _ yy') as (z' & ? & zz' & y'z' & <-).
+    exists z', l. intuition. now transitivity y'.
+  Qed.
+
+  Lemma equ_clos_ss {L} : equ_clos <= t (ss L).
+  Proof.
+    apply Coinduction.
+    intros R t u EQ l t1 TR. cbn in EQ. inv EQ.
+    cbn in *. rewrite Equt in TR.
+    apply HR in TR.
+    destruct TR as (? & ? & ? & ? & ?). subst.
+    exists x. exists x0. intuition.
+    rewrite <- Equu; auto.
+    eapply (f_Tf (ss L)).
+    econstructor; auto; auto.
+  Qed.
+
+(*|
+Aggressively providing instances for rewriting [equ] under all [ss]-related
+contexts.
+|*)
+  #[global] Instance equ_clos_ss_goal L RR :
+    Proper (equ eq ==> equ eq ==> flip impl) (sst L RR).
+  Proof.
+    cbn; intros ? ? eq1 ? ? eq2 H.
+    apply (ft_t equ_clos_ss); econstructor; [eauto | | symmetry; eauto]; assumption.
+  Qed.
+
+  #[global] Instance equ_clos_ss_ctx L RR :
+    Proper (equ eq ==> equ eq ==> impl) (sst L RR).
+  Proof.
+    cbn; intros ? ? eq1 ? ? eq2 H.
+    apply (ft_t equ_clos_ss); econstructor; [symmetry; eauto | | eauto]; assumption.
+  Qed.
+
+  #[global] Instance equ_ssbt_closed_goal {L r} :
+    Proper (equ eq ==> equ eq ==> flip impl) (ssbt L r).
+  Proof.
+    cbn; repeat intro. do 5 red in H1.
+    setoid_rewrite <- H in H1. setoid_rewrite <- H0 in H1.
+    auto.
+  Qed.
+
+  #[global] Instance equ_ssbt_closed_ctx {L r} :
+    Proper (equ eq ==> equ eq ==> impl) (ssbt L r).
+  Proof.
+    cbn; repeat intro. do 5 red in H1.
+    setoid_rewrite H in H1. setoid_rewrite H0 in H1.
+    auto.
+  Qed.
+
+  #[global] Instance equ_clos_ssT_goal L RR f :
+    Proper (equ eq ==> equ eq ==> flip impl) (ssT L f RR).
+  Proof.
+    cbn; intros ? ? eq1 ? ? eq2 H.
+    apply (fT_T equ_clos_ss); econstructor; [eauto | | symmetry; eauto]; assumption.
+  Qed.
+
+  #[global] Instance equ_clos_ssT_ctx L RR f :
+    Proper (equ eq ==> equ eq ==> impl) (ssT L f RR).
+  Proof.
+    cbn; intros ? ? eq1 ? ? eq2 H.
+    apply (fT_T equ_clos_ss); econstructor; [symmetry; eauto | | eauto]; assumption.
+  Qed.
+
+  #[global] Instance equ_clos_ssim_goal L :
+    Proper (equ eq ==> equ eq ==> flip impl) (ssim L).
+  Proof.
+    cbn; intros ? ? eq1 ? ? eq2 H.
+    apply (ft_t equ_clos_ss); econstructor; [eauto | | symmetry; eauto]; assumption.
+  Qed.
+
+  #[global] Instance equ_clos_ssim_ctx L :
+    Proper (equ eq ==> equ eq ==> impl) (ssim L).
+  Proof.
+    cbn; intros ? ? eq1 ? ? eq2 H.
+    apply (ft_t equ_clos_ss); econstructor; [symmetry; eauto | | eauto]; assumption.
+  Qed.
+
+  #[global] Instance equ_ss_closed_goal {L r} : Proper (equ eq ==> equ eq ==> flip impl) (ss L r).
+  Proof.
+    intros t t' tt' u u' uu'; cbn; intros.
+    rewrite tt' in H0. apply H in H0 as (? & ? & ? & ? & ?).
+    eexists; eexists; eauto. rewrite uu'. eauto.
+  Qed.
+
+  #[global] Instance equ_ss_closed_ctx {L r} : Proper (equ eq ==> equ eq ==> impl) (ss L r).
+  Proof.
+    intros t t' tt' u u' uu'; cbn; intros.
+    rewrite <- tt' in H0. apply H in H0 as (? & ? & ? & ? & ?).
+    eexists; eexists; eauto. rewrite <- uu'. eauto.
+  Qed.
+
+(*|
+stuckI and spinI can be simulated by any ctree.
+*)
+
+  Lemma stuckI_ss (R : rel _ _) (t : ctree F D Y) L : ss L R (stuckI : ctree E C X) t.
+  Proof.
+    repeat intro. now apply stuckI_is_stuck in H.
+  Qed.
+
+  Lemma stuckI_ssim (t : ctree F D Y) L : ssim L (stuckI : ctree E C X) t.
+  Proof.
+    intros. step. apply stuckI_ss.
+  Qed.
+
+  Lemma spinI_gen_ss Z (R : rel _ _) (t : ctree F D Y) (x : C Z) L : ss L R (CTree.spinI_gen x : ctree E C X) t.
+  Proof.
+    repeat intro. now apply spinI_gen_is_stuck in H.
+  Qed.
+
+  Lemma spinI_gen_ssim : forall {Z} (c: C Z) (t' : ctree F D Y) L,
+      @CTree.spinI_gen E C X Z c (≲L) t'.
+  Proof.
+    intros. step. apply spinI_gen_ss.
+  Qed.
+
+End ssim_theory.
+
+(*|
+Up-to [bind] context simulations
+----------------------------------
+We have proved in the module [Equ] that up-to bind context is
+a valid enhancement to prove [equ].
+We now prove the same result, but for strong simulation.
+|*)
+
+Section bind.
+  Obligation Tactic := idtac.
+
+ Context {E F C D: Type -> Type} {X X' Y Y': Type}.
+ Context `{HasStuck : C0 -< C} `{HasStuck' : C0 -< D}.
+ Context (L : hrel (@label E) (@label F)).
+
+(*|
+Specialization of [bind_ctx] to a function acting with [ssim] on the bound value,
+and with the argument (pointwise) on the continuation.
+|*)
+  Program Definition bind_ctx_ssim : mon (rel (ctree E C X') (ctree F D Y')) :=
+    {|body := fun R => @bind_ctx E F C D X Y X' Y' (ssim L) (pointwise (fun x y => L (val x) (val y)) R) |}.
+  Next Obligation.
+    intros ?? H. apply leq_bind_ctx. intros ?? H' ?? H''.
+    apply in_bind_ctx. apply H'. intros t t' HS. apply H, H'', HS.
+  Qed.
+
+(*|
+The resulting enhancing function gives a valid up-to technique
+|*)
+  Lemma bind_ctx_ssim_t :
+    (forall l l', L l l' -> is_val l <-> is_val l') ->
+    bind_ctx_ssim <= sst L.
+  Proof.
+    intro HL.
+    apply Coinduction.
+    intros R. apply (leq_bind_ctx _).
+    intros t1 t2 tt k1 k2 kk.
+    step in tt.
+    intros l u STEP.
+    apply trans_bind_inv in STEP as [(H & t' & STEP & EQ) | (v & STEPres & STEP)]; cbn in *.
+    - apply tt in STEP as (u' & l' & STEP & EQ' & ?).
+      eexists. exists l'. split.
+      apply trans_bind_l; eauto.
+      { intro Hl. destruct Hl. apply HL in H0 as [_ ?]. specialize (H0 (Is_val _)). auto. }
+      split; auto.
+      apply (fT_T equ_clos_ss).
+      econstructor; [exact EQ | | reflexivity].
+      apply (fTf_Tf (ss L)).
+      apply in_bind_ctx; auto.
+      intros ? ? ?.
+      apply (b_T (ss L)).
+      red in kk. red. red. now apply kk.
+    - apply tt in STEPres as (u' & ? & STEPres & EQ' & ?).
+      specialize (HL _ _ H) as [? _]. specialize (H0 (Is_val _)). destruct H0.
+      pose proof (trans_val_invT STEPres). subst.
+      pose proof (trans_val_inv STEPres) as EQ.
+      rewrite EQ in STEPres.
+      specialize (kk v x H).
+      apply kk in STEP as (u'' & ? & STEP & EQ'' & ?); cbn in *.
+      eexists. eexists. split.
+      eapply trans_bind_r; eauto.
+      split; auto.
+      eapply (id_T (ss L)); auto.
+  Qed.
+
+End bind.
+
+Import CTree.
+Import CTreeNotations.
+
+(*|
+Expliciting the reasoning rule provided by the up-to principles.
+|*)
+Lemma sst_clo_bind (E F C D: Type -> Type) `{C0 -< C} `{C0 -< D} (X X' Y Y' : Type) L :
+  forall (t1 : ctree E C X) (t2 : ctree F D X') (k1 : X -> ctree E C Y) (k2 : X' -> ctree F D Y') RR,
+		t1 (≲L) t2 ->
+    (forall l l', L l l' -> is_val l <-> is_val l') ->
+    (forall x y, L (val x) (val y) -> (sst L RR) (k1 x) (k2 y)) ->
+    sst L RR (t1 >>= k1) (t2 >>= k2)
+.
+Proof.
+  intros.
+  apply (ft_t (@bind_ctx_ssim_t E F C D X Y X' Y' _ _ L H2)).
+  apply in_bind_ctx; auto.
+Qed.
+
+(*|
+Specializing the congruence principle for [~]
+|*)
+Lemma ssim_clo_bind (E F C D: Type -> Type) `{C0 -< C} `{C0 -< D} (X X' Y Y' : Type) L :
+  forall (t1 : ctree E C X) (t2 : ctree F D X') (k1 : X -> ctree E C Y) (k2 : X' -> ctree F D Y'),
+		t1 (≲L) t2 ->
+    (forall l l', L l l' -> is_val l <-> is_val l') ->
+    (forall x x', L (val x) (val x') -> k1 x (≲L) k2 x') ->
+    t1 >>= k1 (≲L) t2 >>= k2
+.
+Proof.
+  intros.
+  apply (ft_t (@bind_ctx_ssim_t E F C D X Y X' Y' _ _ L H2)).
+  apply in_bind_ctx; auto.
+Qed.
+
+(*|
+And in particular, we can justify rewriting [≲] to the left of a [bind].
+|*)
+Lemma bind_ssim_cong_gen {E F C D X X' Y Y'} `{C0 -< C} `{C0 -< D} RR (L : rel _ _) :
+  forall (t : ctree E C X) (t' : ctree F D X')
+      (k : X -> ctree E C Y) (k' : X' -> ctree F D Y'),
+    (forall l l', L l l' -> is_val l <-> is_val l') ->
+    ssim L t t' ->
+    (forall x x', L (val x) (val x') -> sst L RR (k x) (k' x')) ->
+    sst L RR (CTree.bind t k) (CTree.bind t' k').
+Proof.
+  intros; eapply sst_clo_bind; red in H2; eauto.
+Qed.
+
+Ltac __upto_bind_ssim :=
+  match goal with
+    |- @ssim _ _ _ _ ?X ?X' _ _ _ (CTree.bind (T := ?T) _ _) (CTree.bind (T := ?T') _ _) =>
+      apply ssim_clo_bind
+  | |- body (t (@ss ?E ?F ?C ?D ?X ?Y _ _ ?L)) ?R (CTree.bind (T := ?T) _ _) (CTree.bind (T := ?T') _ _) =>
+      apply (ft_t (@bind_ctx_ssim_t E F C D T T' X Y _ _)), in_bind_ctx
+  | |- body (bt (@ss ?E ?F ?C ?D ?X ?Y _ _ ?L)) ?R (CTree.bind (T := ?T) _ _) (CTree.bind (T := ?T') _ _) =>
+      apply (fbt_bt (@bind_ctx_ssim_t E F C D T T' X Y _ _)), in_bind_ctx
+  end.
+Ltac __upto_bind_eq_ssim :=
+  __upto_bind_ssim; [reflexivity | intros ?].
+
+Ltac __play_ssim := step; cbn; intros ? ? ?TR.
+
+Ltac __play_ssim_in H :=
+  step in H;
+  cbn in H; edestruct H as (? & ? & ?TR & ?EQ & ?);
+  subst; [etrans |].
+
+Ltac __eplay_ssim :=
+  match goal with
+  | h : @ssim ?E ?F ?C ?D ?X ?Y _ _ ?L _ _ |- _ =>
+      __play_ssim_in h
+  end.
+
+#[local] Tactic Notation "play" := __play_ssim.
+#[local] Tactic Notation "play" "in" ident(H) := __play_ssim_in H.
+#[local] Tactic Notation "eplay" := __eplay_ssim.
+
+Section Proof_Rules.
+
+  Context {E F C D : Type -> Type}.
+  Context {HasStuck : C0 -< C} {HasStuck' : C0 -< D}.
+  Context {HasTau : C1 -< C} {HasTau' : C1 -< D}.
+  Context {X X' Y Y' : Type}.
+  Context {L : rel (@label E) (@label F)}.
+
+  Lemma step_ss_ret_gen (x : X) (y : Y) (R : rel _ _) :
+    R stuckI stuckI ->
+    (Proper (equ eq ==> equ eq ==> impl) R) ->
+    L (val x) (val y) ->
+    ss L R (Ret x : ctree E C X) (Ret y : ctree F D Y).
+  Proof.
+    intros Rstuck PROP Lval.
+    cbn; intros ? ? TR; inv_trans; subst.
+    cbn; eexists; eexists; intuition; etrans.
+    now rewrite EQ.
+  Qed.
+
+  Lemma step_ss_ret (x : X) (y : Y) (R : rel _ _) :
+    R stuckI stuckI ->
+    L (val x) (val y) ->
+    ssbt L R (Ret x : ctree E C X) (Ret y : ctree F D Y).
+  Proof.
+    intros.
+    apply step_ss_ret_gen.
+    - step. intros. now apply stuckI_ss.
+    - typeclasses eauto.
+    - apply H0.
+  Qed.
+
+(*|
+The vis nodes are deterministic from the perspective of the labeled transition system,
+stepping is hence symmetric and we can just recover the itree-style rule.
+|*)
+  Lemma step_ss_vis_gen (l : rel _ _) (e : E X) (k : X -> ctree E C Y) (k' : X -> ctree E D Y') (R : rel _ _) :
+    (Proper (equ eq ==> equ eq ==> impl) R) ->
+    (forall x, R (k x) (k' x)) ->
+    (forall x, l (obs e x) (obs e x)) ->
+    ss l R (Vis e k) (Vis e k').
+  Proof.
+    intros PR EQs.
+    intros ? ? ? TR; inv_trans; subst.
+    cbn; eexists; eexists; intuition. rewrite EQ; auto.
+  Qed.
+
+  Lemma step_ss_vis (l : rel _ _) (e : E X) (k : X -> ctree E C Y) (k' : X -> ctree E D Y') (R : rel _ _) :
+    (forall x, sst l R (k x) (k' x)) ->
+    (forall x, l (obs e x) (obs e x)) ->
+    ssbt l R (Vis e k) (Vis e k').
+  Proof.
+    intros * EQ.
+    apply step_ss_vis_gen; auto.
+    typeclasses eauto.
+  Qed.
+
+(*|
+Same goes for visible tau nodes.
+|*)
+   Lemma step_ss_tauV_gen (t : ctree E C X) (t' : ctree F D Y) (R : rel _ _) :
+    (Proper (equ eq ==> equ eq ==> impl) R) ->
+    (R t t') ->
+    L tau tau ->
+    ss L R (tauV t) (tauV t').
+  Proof.
+    intros PR EQs.
+    intros ? ? ? TR; inv_trans; subst.
+    cbn; eexists; eexists; intuition; rewrite EQ; auto.
+  Qed.
+
+  Lemma step_ss_tauV (t : ctree E C X) (t' : ctree F D Y) (R : rel _ _) :
+    L tau tau ->
+    (sst L R t t') ->
+    ssbt L R (tauV t) (tauV t').
+  Proof.
+    intros. apply step_ss_tauV_gen; auto.
+    typeclasses eauto.
+  Qed.
+
+(*|
+When matching visible choices one against another, in general we need to explain how
+we map the branches from the left to the branches to the right.
+A useful special case is the one where the arity coincide and we simply use the identity
+in both directions. We can in this case have [n] rather than [2n] obligations.
+|*)
+
+  Lemma step_ss_choiceV_gen C' Z `{C0 -< C'} (c : C Y) (c' : C' Z)
+    (k : Y -> ctree E C X) (k' : Z -> ctree F C' X') (R : rel _ _) :
+    (Proper (equ eq ==> equ eq ==> impl) R) ->
+    L tau tau ->
+    (forall x, exists y, R (k x) (k' y)) ->
+    ss L R (ChoiceV c k) (ChoiceV c' k').
+  Proof.
+    intros PROP ? EQs.
+    intros ? ? TR; inv_trans; subst.
+    destruct (EQs x) as [z HR].
+    eexists. eexists. intuition.
+    rewrite EQ; eauto.
+  Qed.
+
+  Lemma step_ss_choiceV Z (c : C Y) (c' : D Z)
+    (k : Y -> ctree E C X) (k' : Z -> ctree F D X') (R : rel _ _) :
+    L tau tau ->
+    (forall x, exists y, sst L R (k x) (k' y)) ->
+    ssbt L R (ChoiceV c k) (ChoiceV c' k').
+  Proof.
+    intros ? EQs.
+    apply step_ss_choiceV_gen; auto.
+    typeclasses eauto.
+  Qed.
+
+  Lemma step_ss_choiceV_id_gen (c : C Y)
+    (k : Y -> ctree E C X) (k' : Y -> ctree F C X') (R : rel _ _) :
+    (Proper (equ eq ==> equ eq ==> impl) R) ->
+    L tau tau ->
+    (forall x, R (k x) (k' x)) ->
+    ss L R (ChoiceV c k) (ChoiceV c k').
+  Proof.
+    intros PROP ? EQs.
+    apply step_ss_choiceV_gen; auto.
+    intros x; exists x; auto.
+  Qed.
+
+  Lemma step_ss_choiceV_id (c : C Y)
+    (k : Y -> ctree E C X) (k' : Y -> ctree F C X') (R : rel _ _) :
+    L tau tau ->
+    (forall x, sst L R (k x) (k' x)) ->
+    ssbt L R (ChoiceV c k) (ChoiceV c k').
+  Proof.
+    apply step_ss_choiceV_id_gen.
+    typeclasses eauto.
+  Qed.
+
+(*|
+For invisible nodes, the situation is different: we may kill them, but that execution
+cannot act as going under the guard.
+|*)
+  Lemma step_ss_tauI_gen (t : ctree E C X) (t' : ctree F D Y) (R : rel _ _) :
+    ss L R t t' ->
+    ss L R (tauI t) (tauI t').
+  Proof.
+    intros EQ.
+    intros ? ? TR; inv_trans; subst.
+    apply EQ in TR as (? & ? & ? & ? & ?).
+    eexists; eexists; intuition; subst; [apply trans_tauI; eauto | eauto | eauto].
+  Qed.
+
+  Lemma step_ss_tauI (t : ctree E C X) (t' : ctree F D Y) (R : rel _ _) :
+    ssbt L R t t' ->
+    ssbt L R (tauI t) (tauI t').
+  Proof.
+    apply step_ss_tauI_gen.
+  Qed.
+
+  Lemma step_ss_choiceI_gen' C' Z `{C0 -< C'} (c : C Z)
+    (k : Z -> ctree E C X) (t' : ctree F C' Y) (R : rel _ _) :
+    (forall x, ss L R (k x) t') ->
+    ss L R (ChoiceI c k) t'.
+  Proof.
+    intros EQs.
+    intros ? ? TR; inv_trans; subst.
+    apply EQs in TR; destruct TR as (u' & ? & TR' & EQ' & ?).
+    eexists. eexists. subst. intuition; eauto.
+  Qed.
+
+  Lemma step_ss_choiceI_gen C' Z Z' `{C0 -< C'} (c : C Z) (c' : C' Z')
+    (k : Z -> ctree E C X) (k' : Z' -> ctree F C' Y) (R : rel _ _) :
+    (forall x, exists y, ss L R (k x) (k' y)) ->
+    ss L R (ChoiceI c k) (ChoiceI c' k').
+  Proof.
+    intros EQs.
+    apply step_ss_choiceI_gen'.
+    intros z l t' TR.
+    destruct (EQs z) as [x FF]. cbn in FF.
+    apply FF in TR; destruct TR as (u' & ? & TR' & EQ' & ?).
+    eexists. eexists. subst. intuition; eauto.
+    econstructor. apply TR'.
+  Qed.
+
+  Lemma step_ss_choiceI C' Z Z' `{C0 -< C'} (c : C Z) (c' : C' Z')
+    (k : Z -> ctree E C X) (k' : Z' -> ctree F C' Y) (R : rel _ _) :
+    (forall x, exists y, ssbt L R (k x) (k' y)) ->
+    ssbt L R (ChoiceI c k) (ChoiceI c' k').
+  Proof.
+    apply step_ss_choiceI_gen.
+  Qed.
+
+  Lemma step_ss_choiceI_id_gen Z (c : C Z)
+    (k : Z -> ctree E C X) (k' : Z -> ctree F C Y) (R : rel _ _) :
+    (forall x, ss L R (k x) (k' x)) ->
+    ss L R (ChoiceI c k) (ChoiceI c k').
+  Proof.
+    intros; apply step_ss_choiceI_gen.
+    intros x; exists x; apply H.
+  Qed.
+
+  Lemma step_ss_choiceI_id Z (c : C Z) (k : Z -> ctree E C X) (k' : Z -> ctree F C Y) (R : rel _ _) :
+    (forall x, ssbt L R (k x) (k' x)) ->
+    ssbt L R (ChoiceI c k) (ChoiceI c k').
+  Proof.
+    apply step_ss_choiceI_id_gen.
+  Qed.
+
+End Proof_Rules.
+
+Section WithParams.
+
+  Context {E F C D : Type -> Type}.
+  Context {HasStuck : C0 -< C}.
+  Context {HasTau : C1 -< C}.
+  Context {HasStuck' : C0 -< D}.
+  Context {HasTau' : C1 -< D}.
+  Context (L : rel (@label E) (@label F)).
+
+(*|
+Note that with visible schedules, nary-spins are equivalent only
+if neither are empty, or if both are empty: they match each other's
+tau challenge infinitely often.
+With invisible schedules, they are always equivalent: neither of them
+produce any challenge for the other.
+|*)
+  Lemma spinV_gen_nonempty : forall {Z Z' X Y} (c: C X) (c': D Y) (x: X) (y: Y) (L : rel _ _),
+    L tau tau ->
+    ssim L (@CTree.spinV_gen E C Z X c) (@CTree.spinV_gen F D Z' Y c').
+  Proof.
+    intros.
+    red. coinduction R CH.
+    intros l t' TR.
+    rewrite ctree_eta in TR; cbn in TR.
+    apply trans_choiceV_inv in TR as (_ & EQ & ->).
+    eexists. eexists.
+    rewrite ctree_eta; cbn.
+    split; [econstructor |]. exact y.
+    reflexivity.
+    rewrite EQ; auto.
+  Qed.
+
+(*|
+Inversion principles
+--------------------
+|*)
+  Lemma ssim_ret_inv X Y (r1 : X) (r2 : Y) :
+    (Ret r1 : ctree E C X) (≲L) (Ret r2 : ctree F D Y) -> L (val r1) (val r2).
+  Proof.
+    intro.
+    eplay. inv_trans. now subst.
+  Qed.
+
+  Lemma sbisim_ChoiceV_inv {X Y Z Z'}
+        c1 c2 (k1 : X -> ctree E C Z) (k2 : Y -> ctree F D Z') :
+    ChoiceV c1 k1 (≲L) ChoiceV c2 k2 ->
+    (forall i1, exists i2, k1 i1 (≲L) k2 i2).
+  Proof.
+    intros EQ i1.
+    eplay.
+    inv_trans.
+    eexists; eauto.
+  Qed.
+
+End WithParams.
